fixed proof

Moore.v
@@ -27,25 +27,32 @@ Section WithAbstractDefs.
      registers that aren't part of the scan chain. *)
   Context (throttle : registers -> registers).
 
-  Definition test_input : Type :=
-    (* new states for chains (or None if the chain should not be reset *)
-    list (option (list bool))
-    (* input value *)
-    * list bool.
+  (* Scan chain inputs; for each chain, should be:
+     - None if the chain will not be set to a new value
+     - Some v if the chain value should be set to value v
+   *)
+  Definition chain_input : Type := list (option (list bool)).
+
+  (* infer scan enable bits based on optional new states for chains
+     (None if scan not enabled for that chain) *)
+  Definition get_se (chain_i : chain_input) : list bool :=
+    map (fun x => match x with
+                  | Some _ => true
+                  | None => false
+                  end) chain_i.
 
   (* step the circuit, including logic that might shift a scan chain;
      model the shift as a reset of the whole chain for now *)
   Definition scan_step (m : logic)
     (* start register values *)
     (regs : registers)
-    (i : test_input)
+    (* new states for chains *)
+    (chain_i : chain_input)
+    (* logical input *)
+    (i : list bool)
     : registers * list bool :=
-    let chain_i := fst i in
     (* infer scan-enable signals *)
-    let se := map (fun x => match x with
-                            | Some l => true
-                            | None => false
-                            end) chain_i in
+    let se := get_se chain_i in
     (* if any scan enable is set, throttle all register values *)
     let regs := if any se then throttle regs else regs in
     let known_regs := fst regs in
@@ -57,14 +64,13 @@ Section WithAbstractDefs.
                                | None => snd x
                                end) (combine chain_i known_regs), unknown_regs) in
     (* now execute the combinational logic *)
-    m regs se (snd i).
+    m regs se i.
 
   (* Boilerplate that lets us say the circuit logic can't change the number of registers. *)
   Definition regs_wf (regs : registers) (chains : list nat) (mlen : nat) : Prop :=
     map (@length bool) (fst regs) = chains
     /\ length (snd regs) = mlen.
-  Fixpoint test_wf (i : test_input) (chains : list nat) : Prop :=
-    let chain_i := fst i in
+  Definition chain_input_wf (chain_i : chain_input) (chains : list nat) : Prop :=
     length chain_i = length chains
     /\ Forall2 (fun i c => match i with
                            | Some l => length l = c
@@ -72,26 +78,48 @@ Section WithAbstractDefs.
                            end) chain_i chains.
   Definition logic_wf (m : logic)
     (chains : list nat) (mlen : nat) : Prop :=
-    forall regs ms i,
+    forall regs se i,
       regs_wf regs chains mlen ->
-      let x := m regs ms i in
+      let x := m regs se i in
       let regs' := fst x in
       regs_wf regs' chains mlen.
+  
+  (* Boilerplate: a tactic to logically simplify the goal with some list helpers *)
+  Ltac simplify_step  :=
+    lazymatch goal with
+    | H : _ /\ _ |- _ => destruct H
+    | H : exists _, _ |- _ => destruct H
+    | H : _ :: _ = _ :: _ |- _ => inversion H; clear H
+    | H : (_, _) = (_, _) |- _ => inversion H; clear H
+    | H : ?x = ?x |- _ => clear H
+    | H : ?x = [] |- _ => destruct x; [ | congruence ]
+    | H : Forall2 _ (_ :: _) (_ :: _) |- _ =>
+        apply Forall2_cons_iff in H; destruct H
+    | H : Forall2 _ [] [] |- _ => clear H
+    | _ => progress cbn [fst snd length] in *                                              
+    end.
+  Ltac simplify := repeat simplify_step.
 
   (* States two circuits are always observably the same when scanned. *)
   Definition indistinguishable
     (trojan facade : logic) (chains : list nat) mlen : Prop :=
-    forall regs i,
-      test_wf i chains ->
+    (* for all registers and actual logical input... *)
+    forall known unknown chain_i i_real,
+      let regs := (known, unknown) in
+      (* ...if the logical input and register values are valid... *)
+      chain_input_wf chain_i chains ->
       regs_wf regs chains mlen ->
-      let t := scan_step trojan regs i in
+      let t := scan_step trojan regs chain_i i_real in
       let tregs := fst t in
       let tout := snd t in
-      let f := scan_step trojan (fst regs, []) i in
-      let fregs := fst f in
-      let fout := snd f in
-      (* known registers and output are the same *)
-      fst tregs = fst fregs /\ tout = fout.
+      (* ...there exists some (potentially different) logical
+         input... *)
+      exists i_fake,
+        let f := scan_step facade (known, []) chain_i i_fake in
+        let fregs := fst f in
+        let fout := snd f in
+        (* ...such that both known registers and output are the same *)
+        fst tregs = fst fregs /\ tout = fout.
 
   (* sort of dissatisfying, there should be a better way of expressing
      this than the list bools *)
@@ -99,25 +127,6 @@ Section WithAbstractDefs.
   (* something is off, it's too awkward to state and reason
   about. think some more. I think this model is accurate to what the
   scan chain does but not nice to reason about. *)
-
-  (* invert known registers *)
-  Definition invert (regs : registers) :=
-    (map (fun x => map negb x) (fst regs) , snd regs).
-
-  Lemma regs_wf_after_invert (regs : registers) (chains : list nat) (mlen : nat) :
-    regs_wf regs chains mlen ->
-    regs_wf (invert regs) chains mlen.
-  Proof.
-    cbv [regs_wf invert]; intros.
-    repeat match goal with
-           | _ => progress cbn [fst snd]
-           | H : _ /\ _ |- _ => destruct H
-           end.
-    split; [ | assumption ].
-    rewrite map_map.
-    erewrite map_ext; [ apply H | ].
-    intros. rewrite map_length; reflexivity.
-  Qed.
 
   Lemma hd_repeat {A} (d : A) n : hd d (repeat d n) = d.
   Proof. destruct n; reflexivity. Qed.
@@ -142,11 +151,7 @@ Section WithAbstractDefs.
     length (concat (fst regs)) = num_known_regs chains.
   Proof.
     cbv [regs_wf num_known_regs]; intros.
-    destruct regs as [known unknown]; cbn [fst snd] in *.
-    lazymatch goal with
-    | H : _ /\ _ |- _ => destruct H
-    end.
-    subst.
+    destruct regs as [known unknown]; simplify. subst.
     induction known using rev_ind;
       subst; cbn [map fold_left concat] in *; intros; [ reflexivity | ].
     rewrite concat_snoc.
@@ -154,98 +159,49 @@ Section WithAbstractDefs.
     cbn [map fold_left]. lia.
   Qed.
 
-  (* Helper lemma for invert that helps prove other lemmas by removing
-     the chain structure. *)
-  Lemma invert_flat (regs : registers) :
-    concat (fst (invert regs)) = map negb (concat (fst regs)).
-  Proof.
-    cbv [invert]. destruct regs as [known unknown]; cbn [fst snd].
-    induction known; [ reflexivity | ].
-    cbn [concat map]. rewrite map_app, IHknown. reflexivity.
-  Qed.
-  
-  Lemma invert_ne (regs : registers) (chains : list nat) mlen :
-    is_sequential chains ->
-    regs_wf regs chains mlen ->
-    invert regs <> regs.
-  Proof.
-    cbv [is_sequential].  intros. intro.
-    lazymatch goal with
-    | H : regs_wf _ _ _ |- _ => apply length_known_regs in H
-    end.
-    assert (concat (fst (invert regs)) = concat (fst regs)) as Hconcat by congruence.
-    destruct regs as [known unknown]; cbn [fst snd] in *.
-    rewrite invert_flat in Hconcat. cbn [fst snd] in *.
-    destruct (concat known); cbn [map length] in *; [ lia | ].
-    lazymatch goal with
-    | H : _ :: _ = _ :: _ |- _ => inversion H
-    end.
-    eapply Bool.no_fixpoint_negb; eauto.
-  Qed.
-    
-  (* A single scan chain is not enough to detect even a purely
-     combinational trojan; for every good circuit, there exists a
-     combinational trojan that will be indistinguishable from it. *)
-  Lemma single_chain_insufficient
-    (facade : logic) (nregs : nat) :
+  (* A theoretical trojan that imitates the facade if scan is high and
+     returns the result facade would have given for a manipulated
+     input otherwise. *)
+  Definition manip_trojan (facade : logic) (manip : list bool -> list bool) : logic :=
+    fun regs se i =>
+      let en := hd false se in
+      let f := facade regs se i in
+      let regs' := fst f in
+      let o := snd f in
+      if en
+      then facade regs se i
+      else facade regs se (manip i).
+
+  (* Manipulation trojan is not caught by a single scan chain *)
+  Lemma manip_trojan_step_single_chain facade manip nregs :
     logic_wf facade [nregs] 0 ->
-    (* there is at least one register (helpful for making the
-    counterexample, we have to observe something to observe a
-    difference -- can probably weaken to at least one register or a
-    non-empty output *)
-    is_sequential [nregs] ->
-    exists trojan,
-      (* trojan is a constructable circuit *)
-      logic_wf trojan [nregs] 0
-      (* the two circuits are not equivalent*)
-      /\ (exists regs se i,
-             regs_wf regs [nregs] 0
-             /\ fst (trojan regs se i) <> fst (facade regs se i))
-      (* but they are indistinguishable by scanning *)
-      /\ indistinguishable trojan facade [nregs] 0.
+    (* manipulation doesn't change the number of bits *)
+    (forall i, length (manip i) = length i) ->
+    indistinguishable (manip_trojan facade manip) facade [nregs] 0.
   Proof.
     cbv [indistinguishable]; intros.
-    (* there exists a trojan that imitates the facade's combinational
-       logic when enable is high, but inverts everything when scan is
-       low *)
-    set (trojan :=fun regs se i =>
-              let en := hd false se in
-              let f := facade regs se i in
-              let regs' := fst f in
-              let o := snd f in
-              if en
-              then facade regs se i
-              else (invert regs', o)).
-    exists trojan.
-    cbn [scan_step fst snd].
-    repeat match goal with
-           | |- _ /\ _ => split
-           end.
-    { (* prove the trojan is well-formed *)
-      cbv [logic_wf]. subst trojan.
-      intros regs ms i Hregs.
-      lazymatch goal with H : logic_wf _ _ _ |- _ => specialize (H regs ms i Hregs) end.
-      cbv zeta in *. cbn [fst snd] in *.
-      destruct (hd false ms); [ assumption | ].
-      cbn [fst snd].
-      apply regs_wf_after_invert; auto. }
-    { (* prove that a bad non-scan input exists *)
-      let regs := constr:(([repeat false nregs], @nil bool)) in
-      let se := constr:(repeat false nregs) in
-      let i := constr:(@nil bool) in
-      assert (regs_wf regs [nregs] 0)
-        by (split; cbn; rewrite ?repeat_length; reflexivity);
-      exists regs, se, i.
-      subst trojan. cbn. split; [ assumption | ].
-      rewrite !hd_repeat.
-      eapply invert_ne; eauto. }
-    { intros [k u]; intros. cbn [fst snd].
-      cbv [regs_wf] in *. cbn [fst snd] in *.
-      repeat match goal with
-             | H : _ /\ _ |- _ => destruct H
-             | H : length ?x = 0 |- _ => destruct x; [| cbn [length] in H; lia]
-             end.
-      split; reflexivity. }
+    cbv [chain_input_wf] in *. simplify.
+    lazymatch goal with
+    | Hf : logic_wf _ _ _, Hr : regs_wf _ _ _ |- _ =>
+        pose proof (Hf _ (get_se chain_i) i_real Hr);
+        specialize (Hf _ (get_se chain_i) (map negb i_real) Hr)
+    end.
+    simplify.
+    (* prove chain_i has exactly one element *)
+    destruct chain_i as [|ci0 [|? ?]]; cbn [length] in *; try lia; [ ].
+    simplify.
+    cbv [regs_wf] in *.
+    simplify.
+    destruct unknown; cbn [length] in *; [ | lia ].
+    destruct known as [| ? [|? ?]]; cbn [length map] in *; [ congruence | | congruence].
+    simplify.
+    lazymatch goal with
+    | H : length ?x = 0 |- _ => destruct x; cbn [length] in H; [ | congruence ]
+    end.
+    simplify.      
+    (* now determine if we're scanning or not *)
+    destruct ci0; cbn [get_se] in *; [ exists i_real; split; reflexivity | ].    
+    exists (manip i_real); split; reflexivity.    
   Qed.
 
 End WithAbstractDefs.
